forgot file

iodiv/DivFreeTauDM.Test.fst
@@ -29,10 +29,10 @@ let lem_spec_to_loop
   (inv0 : trace -> Type0)
   (pre0_inv0 : squash (forall h lt. pre0 h /\ inv0 lt ==> pre0 (rev_acc lt h))) :
   Lemma (
-    let body0 : iwp a = iprepost pre0 (fun h r -> terminates r /\ inv0 (_trace r)) in
+    let body0 : iwp a = iprepost pre0 (fun h r -> terminates r /\ inv0 (ret_trace r)) in
     let loop0 : iwp unit = iprepost pre0 (fun h r -> diverges r /\ repeat_inv_post inv0 r) in
     i_iter (lift_i body0) () `ile` loop0) =
-  let body0 : iwp a = iprepost pre0 (fun h r -> terminates r /\ inv0 (_trace r)) in
+  let body0 : iwp a = iprepost pre0 (fun h r -> terminates r /\ inv0 (ret_trace r)) in
   let loop0 = iprepost pre0 (fun h r -> diverges r /\ repeat_inv_post inv0 r) in
   let body' = lift_i body0 in
   let body_inv = repeat_body_inv #unit (fun _ -> pre0) inv0 in
@@ -49,9 +49,9 @@ let lem_body_to_loop
   (#pre0 : trace -> Type0)
   (#inv0 : trace -> Type0)
   (#pre0_inv0 : squash (forall h lt. pre0 h /\ inv0 lt ==> pre0 (rev_acc lt h))) 
-  (f : iodiv_dm a (iprepost pre0 (fun h r -> terminates r /\ inv0 (_trace r)))) :
+  (f : iodiv_dm a (iprepost pre0 (fun h r -> terminates r /\ inv0 (ret_trace r)))) :
   Lemma (
-    let body0 : iwp a = iprepost pre0 (fun h r -> terminates r /\ inv0 (_trace r)) in
+    let body0 : iwp a = iprepost pre0 (fun h r -> terminates r /\ inv0 (ret_trace r)) in
     let loop0 : iwp unit = iprepost pre0 (fun h r -> diverges r /\ repeat_inv_post inv0 r) in
     i_iter (lift_i body0) () `ile` loop0) =
   lem_spec_to_loop a pre0 inv0 pre0_inv0
@@ -63,12 +63,21 @@ let dm_loop1 (fd:file_descr) : iodiv_dm unit (iloop1 fd) =
   iodiv_repeat (dm_body1 fd)
 
 (** ** Test print 0 1 **)
-
-(** What the actual **** **)
-let dm_body2 : iodiv_dm unit (iprepost (fun _ -> True) (fun h r -> terminates r /\ _trace r == [EPrint "0";EPrint "1"] /\ False)) = 
+let body2 : m io_sig unit = 
   (m_bind (m_call Print "0") (fun () -> m_call Print "1"))
 
-let iloop2 : iwp unit = iprepost (fun _ -> True) (fun h r -> diverges r /\ False) //repeat_inv_post (fun lt -> lt == [EPrint "0"; EPrint "3:"]) r)
+let ibody2 : iwp unit =
+  iprepost (fun _ -> True) (fun h r -> terminates r /\ ret_trace r == [EPrint "0";EPrint "1"])
 
-let dm_loop2 () : iodiv_dm unit iloop2  =
-  iodiv_repeat dm_body2
+let dm_body2 () : iodiv_dm unit ibody2 = 
+  let d : iodiv_dm unit (i_bind_alt (iodiv_act Print "0") (fun _ -> iodiv_act Print "1")) = 
+    (iodiv_bind _ _ _ _ (iodiv_call Print "0") (fun () -> iodiv_call Print "1")) in
+  assume ((i_bind_alt (iodiv_act Print "0") (fun _ -> iodiv_act Print "1")) `ile` ibody2);
+  iodiv_subcomp _ _ _ d
+
+let iloop2 : iwp unit = iprepost (fun _ -> True) (fun h r -> diverges r /\ repeat_inv_post (fun lt -> lt == [EPrint "0"; EPrint "1"]) r)
+
+let dm_loop2 () : iodiv_dm unit iloop2 =
+  let d : iodiv_dm unit (i_iter (lift_i ibody2) ()) = iodiv_repeat (dm_body2 ()) in
+  lem_body_to_loop #_ #(fun _ -> True) #(fun lt -> lt == [EPrint "0"; EPrint "1"]) (dm_body2 ());
+  iodiv_subcomp _ _ _ d
